src/dafny/beacon/helpers/Math.dfy
@@ -33,47 +33,35 @@ module  Math
      *  @param       n   A natural number
      *  @return     `x` 
      */    
-    method  integer_squareroot(n:uint64) returns (x:uint64)
+    method  integer_squareroot(n:uint64) returns (x:uint64) 
     requires n < 0xFFFFFFFFFFFFFFFF;
     ensures power(x as nat,2) <= n as nat;
-    ensures !(exists x' {:trigger power(x' as nat,2)} :: x'>x && power(x' as nat,2) <= n as nat)
+    ensures !(exists x' {:trigger power(x' as nat,2)} :: 
+                    x'>x && power(x' as nat,2) <= n as nat)
     {
-        reveal_power();
         x:=n;    
-        var y :=(x+1)/2;
+        var y:uint64 :=(x+1)/2;
 
         while(y<x)
             decreases x
-            invariant y >= x <==> x as nat *x as nat <= n as nat;
+            invariant y < x <==> power(x as nat,2) > n as nat;
             invariant power(y as nat +1,2) > n as nat;
             invariant power(x as nat +1,2) > n as nat;
             invariant y <= 0x7FFFFFFFFFFFFFFF;
-        {
+        {   
             LemmaMaxForYDivByX(y as nat,n as nat);
-            
+
             x := y;          
 
             y:=(x+n/x)/2;
             
-            assert power(x as nat,2) > n as nat <==> y < x by 
-            {
-                LemmaYStrictlyLessThanXIff(x as nat,n as nat);
-            }
-
-            assert power(y as nat +1,2) > n as nat by
-            {
-                LemmaSquareYPlusOneGreaterThanX(x as nat,n as nat);
-            }
+            LemmaLoopInvariants(x as nat,n as nat);
         }
 
-        forall i {:trigger power(i as nat,2)} | i > x
-        ensures power(i as nat,2) > n as nat
-        {
-            lemma_power_increases((x + 1) as nat,i as nat,2);
-        }
+        LemmaSquareIsMonotonic(x as nat +1);
 
         return x;
-    }    
+    }   
     
     /**
      * Computes the exclusive-or of two `Bytes32` values
@@ -106,7 +94,6 @@ module  Math
     requires length <= 8
     ensures |int_to_bytes(n,length)| == length as int
     {
-        reveal_power();
         if(length == 0) then
             []
         else
@@ -127,7 +114,6 @@ module  Math
     requires |s| <= 8 
     ensures bytes_to_int(s) as nat < power(256,|s|)
     {
-        reveal_power();
         if(|s| == 0) then
             0
         else
